saturn/spsc_queue_queue → saturn/spsc_bqueue.

theories/saturn/spsc_bqueue.v
@@ -53,11 +53,11 @@ Implicit Types vs hist : list val.
 )(in custom zebre_field
 ).
 
-Definition spsc_queue_create : val :=
+Definition spsc_bqueue_create : val :=
   λ: "sz",
     { array_make "sz" §None; #0; #0; #0; #0 }.
 
-#[local] Definition spsc_queue_push_aux : val :=
+#[local] Definition spsc_bqueue_push_aux : val :=
   λ: "t" "data" "back",
     let: "sz" := array_size "data" in
     let: "front_cache" := "t".{front_cache} in
@@ -68,11 +68,11 @@ Definition spsc_queue_create : val :=
       "t" <-{front_cache} "front" ;;
       "back" < "front" + "sz"
     ).
-Definition spsc_queue_push : val :=
+Definition spsc_bqueue_push : val :=
   λ: "t" "v",
     let: "data" := "t".{data} in
     let: "back" := "t".{back} in
-    if: spsc_queue_push_aux "t" "data" "back" then (
+    if: spsc_bqueue_push_aux "t" "data" "back" then (
       array_cset "data" "back" ‘Some{ "v" } ;;
       "t" <-{back} #1 + "back" ;;
       #false
@@ -80,7 +80,7 @@ Definition spsc_queue_push : val :=
       #true
     ).
 
-#[local] Definition spsc_queue_pop_aux : val :=
+#[local] Definition spsc_bqueue_pop_aux : val :=
   λ: "t" "front",
     let: "back_cache" := "t".{back_cache} in
     if: "front" < "back_cache" then (
@@ -90,10 +90,10 @@ Definition spsc_queue_push : val :=
       "t" <-{back_cache} "back" ;;
       "front" < "back"
     ).
-Definition spsc_queue_pop : val :=
+Definition spsc_bqueue_pop : val :=
   λ: "t",
     let: "front" := "t".{front} in
-    if: spsc_queue_pop_aux "t" "front" then (
+    if: spsc_bqueue_pop_aux "t" "front" then (
       let: "data" := "t".{data} in
       let: "res" := array_cget "data" "front" in
       array_cset "data" "front" §None ;;
@@ -103,364 +103,364 @@ Definition spsc_queue_pop : val :=
       §None
     ).
 
-Class SpscQueueG Σ `{zebre_G : !ZebreG Σ} := {
-  #[local] spsc_queue_G_model_G :: TwinsG Σ (listO valO) ;
-  #[local] spsc_queue_G_history_G :: MonoListG Σ val ;
-  #[local] spsc_queue_G_ctl_G :: AuthNatMaxG Σ ;
-  #[local] spsc_queue_G_region_G :: ExclG Σ unitO ;
+Class SpscBqueueG Σ `{zebre_G : !ZebreG Σ} := {
+  #[local] spsc_bqueue_G_model_G :: TwinsG Σ (listO valO) ;
+  #[local] spsc_bqueue_G_history_G :: MonoListG Σ val ;
+  #[local] spsc_bqueue_G_ctl_G :: AuthNatMaxG Σ ;
+  #[local] spsc_bqueue_G_region_G :: ExclG Σ unitO ;
 }.
 
-Definition spsc_queue_Σ := #[
+Definition spsc_bqueue_Σ := #[
   twins_Σ (listO valO) ;
   mono_list_Σ val ;
   auth_nat_max_Σ ;
   excl_Σ unitO
 ].
-Lemma subG_spsc_queue_Σ Σ `{zebre_G : !ZebreG Σ} :
-  subG spsc_queue_Σ Σ →
-  SpscQueueG Σ.
+Lemma subG_spsc_bqueue_Σ Σ `{zebre_G : !ZebreG Σ} :
+  subG spsc_bqueue_Σ Σ →
+  SpscBqueueG Σ.
 Proof.
   solve_inG.
 Qed.
 
-Section spsc_queue_G.
-  Context `{spsc_queue_G : SpscQueueG Σ}.
+Section spsc_bqueue_G.
+  Context `{spsc_bqueue_G : SpscBqueueG Σ}.
 
-  Record spsc_queue_meta := {
-    spsc_queue_meta_model : gname ;
-    spsc_queue_meta_history : gname ;
-    spsc_queue_meta_producer_ctl : gname ;
-    spsc_queue_meta_producer_region : gname ;
-    spsc_queue_meta_consumer_ctl : gname ;
-    spsc_queue_meta_consumer_region : gname ;
+  Record spsc_bqueue_meta := {
+    spsc_bqueue_meta_model : gname ;
+    spsc_bqueue_meta_history : gname ;
+    spsc_bqueue_meta_producer_ctl : gname ;
+    spsc_bqueue_meta_producer_region : gname ;
+    spsc_bqueue_meta_consumer_ctl : gname ;
+    spsc_bqueue_meta_consumer_region : gname ;
   }.
-  Implicit Types γ : spsc_queue_meta.
+  Implicit Types γ : spsc_bqueue_meta.
 
-  #[local] Instance spsc_queue_meta_eq_dec : EqDecision spsc_queue_meta :=
+  #[local] Instance spsc_bqueue_meta_eq_dec : EqDecision spsc_bqueue_meta :=
     ltac:(solve_decision).
-  #[local] Instance spsc_queue_meta_countable :
-    Countable spsc_queue_meta.
+  #[local] Instance spsc_bqueue_meta_countable :
+    Countable spsc_bqueue_meta.
   Proof.
     pose encode γ := (
-      γ.(spsc_queue_meta_model),
-      γ.(spsc_queue_meta_history),
-      γ.(spsc_queue_meta_producer_ctl),
-      γ.(spsc_queue_meta_producer_region),
-      γ.(spsc_queue_meta_consumer_ctl),
-      γ.(spsc_queue_meta_consumer_region)
+      γ.(spsc_bqueue_meta_model),
+      γ.(spsc_bqueue_meta_history),
+      γ.(spsc_bqueue_meta_producer_ctl),
+      γ.(spsc_bqueue_meta_producer_region),
+      γ.(spsc_bqueue_meta_consumer_ctl),
+      γ.(spsc_bqueue_meta_consumer_region)
     ).
     pose decode := λ '(γ_model, γ_history, γ_producer_ctl, γ_producer_region, γ_consumer_ctl, γ_consumer_region), {|
-      spsc_queue_meta_model := γ_model ;
-      spsc_queue_meta_history := γ_history ;
-      spsc_queue_meta_producer_ctl := γ_producer_ctl ;
-      spsc_queue_meta_producer_region := γ_producer_region ;
-      spsc_queue_meta_consumer_ctl := γ_consumer_ctl ;
-      spsc_queue_meta_consumer_region := γ_consumer_region ;
+      spsc_bqueue_meta_model := γ_model ;
+      spsc_bqueue_meta_history := γ_history ;
+      spsc_bqueue_meta_producer_ctl := γ_producer_ctl ;
+      spsc_bqueue_meta_producer_region := γ_producer_region ;
+      spsc_bqueue_meta_consumer_ctl := γ_consumer_ctl ;
+      spsc_bqueue_meta_consumer_region := γ_consumer_region ;
     |}.
     refine (inj_countable' encode decode _). intros []. done.
   Qed.
 
-  #[local] Definition spsc_queue_model₁' γ_model vs :=
+  #[local] Definition spsc_bqueue_model₁' γ_model vs :=
     twins_twin2 γ_model vs.
-  #[local] Definition spsc_queue_model₁ γ vs :=
-    spsc_queue_model₁' γ.(spsc_queue_meta_model) vs.
-  #[local] Definition spsc_queue_model₂' γ_model vs :=
+  #[local] Definition spsc_bqueue_model₁ γ vs :=
+    spsc_bqueue_model₁' γ.(spsc_bqueue_meta_model) vs.
+  #[local] Definition spsc_bqueue_model₂' γ_model vs :=
     twins_twin1 γ_model (DfracOwn 1) vs.
-  #[local] Definition spsc_queue_model₂ γ vs :=
-    spsc_queue_model₂' γ.(spsc_queue_meta_model) vs.
+  #[local] Definition spsc_bqueue_model₂ γ vs :=
+    spsc_bqueue_model₂' γ.(spsc_bqueue_meta_model) vs.
 
-  #[local] Definition spsc_queue_history_auth' γ_history hist :=
+  #[local] Definition spsc_bqueue_history_auth' γ_history hist :=
     mono_list_auth γ_history (DfracOwn 1) hist.
-  #[local] Definition spsc_queue_history_auth γ hist :=
-    spsc_queue_history_auth' γ.(spsc_queue_meta_history) hist.
-  #[local] Definition spsc_queue_history_elem γ i v :=
-    mono_list_elem γ.(spsc_queue_meta_history) i v.
+  #[local] Definition spsc_bqueue_history_auth γ hist :=
+    spsc_bqueue_history_auth' γ.(spsc_bqueue_meta_history) hist.
+  #[local] Definition spsc_bqueue_history_elem γ i v :=
+    mono_list_elem γ.(spsc_bqueue_meta_history) i v.
 
-  #[local] Definition spsc_queue_producer_ctl₁' γ_producer_ctl back :=
+  #[local] Definition spsc_bqueue_producer_ctl₁' γ_producer_ctl back :=
     auth_nat_max_auth γ_producer_ctl (DfracOwn (1/2)) back.
-  #[local] Definition spsc_queue_producer_ctl₁ γ back :=
-    spsc_queue_producer_ctl₁' γ.(spsc_queue_meta_producer_ctl) back.
-  #[local] Definition spsc_queue_producer_ctl₂' γ_producer_ctl back :=
+  #[local] Definition spsc_bqueue_producer_ctl₁ γ back :=
+    spsc_bqueue_producer_ctl₁' γ.(spsc_bqueue_meta_producer_ctl) back.
+  #[local] Definition spsc_bqueue_producer_ctl₂' γ_producer_ctl back :=
     auth_nat_max_auth γ_producer_ctl (DfracOwn (1/2)) back.
-  #[local] Definition spsc_queue_producer_ctl₂ γ back :=
-    spsc_queue_producer_ctl₂' γ.(spsc_queue_meta_producer_ctl) back.
-  #[local] Definition spsc_queue_back_lb γ back :=
-    auth_nat_max_lb γ.(spsc_queue_meta_producer_ctl) back.
+  #[local] Definition spsc_bqueue_producer_ctl₂ γ back :=
+    spsc_bqueue_producer_ctl₂' γ.(spsc_bqueue_meta_producer_ctl) back.
+  #[local] Definition spsc_bqueue_back_lb γ back :=
+    auth_nat_max_lb γ.(spsc_bqueue_meta_producer_ctl) back.
 
-  #[local] Definition spsc_queue_producer_region' γ_producer_region :=
+  #[local] Definition spsc_bqueue_producer_region' γ_producer_region :=
     excl γ_producer_region ().
-  #[local] Definition spsc_queue_producer_region γ :=
-    spsc_queue_producer_region' γ.(spsc_queue_meta_producer_region).
+  #[local] Definition spsc_bqueue_producer_region γ :=
+    spsc_bqueue_producer_region' γ.(spsc_bqueue_meta_producer_region).
 
-  #[local] Definition spsc_queue_consumer_ctl₁' γ_consumer_ctl front :=
+  #[local] Definition spsc_bqueue_consumer_ctl₁' γ_consumer_ctl front :=
     auth_nat_max_auth γ_consumer_ctl (DfracOwn (1/2)) front.
-  #[local] Definition spsc_queue_consumer_ctl₁ γ front :=
-    spsc_queue_consumer_ctl₁' γ.(spsc_queue_meta_consumer_ctl) front.
-  #[local] Definition spsc_queue_consumer_ctl₂' γ_consumer_ctl front :=
+  #[local] Definition spsc_bqueue_consumer_ctl₁ γ front :=
+    spsc_bqueue_consumer_ctl₁' γ.(spsc_bqueue_meta_consumer_ctl) front.
+  #[local] Definition spsc_bqueue_consumer_ctl₂' γ_consumer_ctl front :=
     auth_nat_max_auth γ_consumer_ctl (DfracOwn (1/2)) front.
-  #[local] Definition spsc_queue_consumer_ctl₂ γ front :=
-    spsc_queue_consumer_ctl₂' γ.(spsc_queue_meta_consumer_ctl) front.
-  #[local] Definition spsc_queue_front_lb γ front :=
-    auth_nat_max_lb γ.(spsc_queue_meta_consumer_ctl) front.
+  #[local] Definition spsc_bqueue_consumer_ctl₂ γ front :=
+    spsc_bqueue_consumer_ctl₂' γ.(spsc_bqueue_meta_consumer_ctl) front.
+  #[local] Definition spsc_bqueue_front_lb γ front :=
+    auth_nat_max_lb γ.(spsc_bqueue_meta_consumer_ctl) front.
 
-  #[local] Definition spsc_queue_consumer_region' γ_consumer_region :=
+  #[local] Definition spsc_bqueue_consumer_region' γ_consumer_region :=
     excl γ_consumer_region ().
-  #[local] Definition spsc_queue_consumer_region γ :=
-    spsc_queue_consumer_region' γ.(spsc_queue_meta_consumer_region).
+  #[local] Definition spsc_bqueue_consumer_region γ :=
+    spsc_bqueue_consumer_region' γ.(spsc_bqueue_meta_consumer_region).
 
-  #[local] Definition spsc_queue_inv_inner l γ sz data : iProp Σ :=
+  #[local] Definition spsc_bqueue_inv_inner l γ sz data : iProp Σ :=
     ∃ front back vs hist,
     ⌜back = (front + length vs)%nat ∧ back ≤ front + sz⌝ ∗
     ⌜length hist = back ∧ vs = drop front hist⌝ ∗
     l.[front] ↦ #front ∗
-    spsc_queue_consumer_ctl₂ γ front ∗
+    spsc_bqueue_consumer_ctl₂ γ front ∗
     l.[back] ↦ #back ∗
-    spsc_queue_producer_ctl₂ γ back ∗
-    spsc_queue_model₂ γ vs ∗
-    spsc_queue_history_auth γ hist ∗
+    spsc_bqueue_producer_ctl₂ γ back ∗
+    spsc_bqueue_model₂ γ vs ∗
+    spsc_bqueue_history_auth γ hist ∗
     ( array_cslice data sz front (DfracOwn 1) ((λ v, ’Some{ v }) <$> take 1 vs)
-    ∨ spsc_queue_consumer_region γ
+    ∨ spsc_bqueue_consumer_region γ
     ) ∗
     array_cslice data sz (S front) (DfracOwn 1) ((λ v, ’Some{ v }) <$> drop 1 vs) ∗
     ( array_cslice data sz back (DfracOwn 1) (if decide (back = front + sz) then [] else [§None])
-    ∨ spsc_queue_producer_region γ
+    ∨ spsc_bqueue_producer_region γ
     ) ∗
     array_cslice data sz (S back) (DfracOwn 1) (replicate (sz - (back - front) - 1) §None).
-  Definition spsc_queue_inv t ι sz : iProp Σ :=
+  Definition spsc_bqueue_inv t ι sz : iProp Σ :=
     ∃ l γ data,
     ⌜t = #l⌝ ∗
     meta l nroot γ ∗
     l.[data] ↦□ data ∗
-    inv ι (spsc_queue_inv_inner l γ sz data).
+    inv ι (spsc_bqueue_inv_inner l γ sz data).
 
-  Definition spsc_queue_model t vs : iProp Σ :=
+  Definition spsc_bqueue_model t vs : iProp Σ :=
     ∃ l γ,
     ⌜t = #l⌝ ∗
     meta l nroot γ ∗
-    spsc_queue_model₁ γ vs.
+    spsc_bqueue_model₁ γ vs.
 
-  Definition spsc_queue_producer t : iProp Σ :=
+  Definition spsc_bqueue_producer t : iProp Σ :=
     ∃ l γ front_cache back,
     ⌜t = #l⌝ ∗
     meta l nroot γ ∗
     l.[front_cache] ↦ #front_cache ∗
-    spsc_queue_producer_ctl₁ γ back ∗
-    spsc_queue_producer_region γ ∗
-    spsc_queue_front_lb γ front_cache.
+    spsc_bqueue_producer_ctl₁ γ back ∗
+    spsc_bqueue_producer_region γ ∗
+    spsc_bqueue_front_lb γ front_cache.
 
-  Definition spsc_queue_consumer t : iProp Σ :=
+  Definition spsc_bqueue_consumer t : iProp Σ :=
     ∃ l γ front back_cache,
     ⌜t = #l⌝ ∗
     meta l nroot γ ∗
     l.[back_cache] ↦ #back_cache ∗
-    spsc_queue_consumer_ctl₁ γ front ∗
-    spsc_queue_consumer_region γ ∗
-    spsc_queue_back_lb γ back_cache.
+    spsc_bqueue_consumer_ctl₁ γ front ∗
+    spsc_bqueue_consumer_region γ ∗
+    spsc_bqueue_back_lb γ back_cache.
 
-  #[global] Instance spsc_queue_inv_persistent t ι sz :
-    Persistent (spsc_queue_inv t ι sz).
+  #[global] Instance spsc_bqueue_inv_persistent t ι sz :
+    Persistent (spsc_bqueue_inv t ι sz).
   Proof.
     apply _.
   Qed.
-  #[global] Instance spsc_queue_model_timeless t vs :
-    Timeless (spsc_queue_model t vs).
+  #[global] Instance spsc_bqueue_model_timeless t vs :
+    Timeless (spsc_bqueue_model t vs).
   Proof.
     apply _.
   Qed.
-  #[global] Instance spsc_queue_producer_timeless t :
-    Timeless (spsc_queue_producer t).
+  #[global] Instance spsc_bqueue_producer_timeless t :
+    Timeless (spsc_bqueue_producer t).
   Proof.
     apply _.
   Qed.
-  #[global] Instance spsc_queue_consumer_timeless t :
-    Timeless (spsc_queue_consumer t).
+  #[global] Instance spsc_bqueue_consumer_timeless t :
+    Timeless (spsc_bqueue_consumer t).
   Proof.
     apply _.
   Qed.
 
-  #[local] Lemma spsc_queue_model_alloc :
+  #[local] Lemma spsc_bqueue_model_alloc :
     ⊢ |==>
       ∃ γ_model,
-      spsc_queue_model₁' γ_model [] ∗
-      spsc_queue_model₂' γ_model [].
+      spsc_bqueue_model₁' γ_model [] ∗
+      spsc_bqueue_model₂' γ_model [].
   Proof.
-    iMod (twins_alloc' (twins_G := spsc_queue_G_model_G) []) as "(%γ_model & Hmodel₁ & Hmodel₂)".
+    iMod (twins_alloc' (twins_G := spsc_bqueue_G_model_G) []) as "(%γ_model & Hmodel₁ & Hmodel₂)".
     iSteps.
   Qed.
-  #[local] Lemma spsc_queue_model_agree γ model1 model2 :
-    spsc_queue_model₁ γ model1 -∗
-    spsc_queue_model₂ γ model2 -∗
+  #[local] Lemma spsc_bqueue_model_agree γ model1 model2 :
+    spsc_bqueue_model₁ γ model1 -∗
+    spsc_bqueue_model₂ γ model2 -∗
     ⌜model1 = model2⌝.
   Proof.
     iIntros "Hmodel₁ Hmodel₂".
     iDestruct (twins_agree_L with "Hmodel₂ Hmodel₁") as %->.
     iSteps.
   Qed.
-  #[local] Lemma spsc_queue_model_update {γ model1 model2} model :
-    spsc_queue_model₁ γ model1 -∗
-    spsc_queue_model₂ γ model2 ==∗
-      spsc_queue_model₁ γ model ∗
-      spsc_queue_model₂ γ model.
+  #[local] Lemma spsc_bqueue_model_update {γ model1 model2} model :
+    spsc_bqueue_model₁ γ model1 -∗
+    spsc_bqueue_model₂ γ model2 ==∗
+      spsc_bqueue_model₁ γ model ∗
+      spsc_bqueue_model₂ γ model.
   Proof.
     iIntros "Hmodel₁ Hmodel₂".
     iMod (twins_update' with "Hmodel₂ Hmodel₁") as "(Hmodel₂ & Hmodel₁)".
     iSteps.
   Qed.
 
-  #[local] Lemma spsc_queue_history_alloc :
+  #[local] Lemma spsc_bqueue_history_alloc :
     ⊢ |==>
       ∃ γ_history,
-      spsc_queue_history_auth' γ_history [].
+      spsc_bqueue_history_auth' γ_history [].
   Proof.
     apply mono_list_alloc.
   Qed.
-  #[local] Lemma spsc_queue_history_elem_get {γ hist} i v :
+  #[local] Lemma spsc_bqueue_history_elem_get {γ hist} i v :
     hist !! i = Some v →
-    spsc_queue_history_auth γ hist ⊢
-    spsc_queue_history_elem γ i v.
+    spsc_bqueue_history_auth γ hist ⊢
+    spsc_bqueue_history_elem γ i v.
   Proof.
     setoid_rewrite mono_list_lb_get. apply mono_list_elem_get.
   Qed.
-  #[local] Lemma spsc_queue_history_agree γ hist i v :
-    spsc_queue_history_auth γ hist -∗
-    spsc_queue_history_elem γ i v -∗
+  #[local] Lemma spsc_bqueue_history_agree γ hist i v :
+    spsc_bqueue_history_auth γ hist -∗
+    spsc_bqueue_history_elem γ i v -∗
     ⌜hist !! i = Some v⌝.
   Proof.
     apply mono_list_lookup.
   Qed.
-  #[local] Lemma spsc_queue_history_update {γ hist} v :
-    spsc_queue_history_auth γ hist ⊢ |==>
-    spsc_queue_history_auth γ (hist ++ [v]).
+  #[local] Lemma spsc_bqueue_history_update {γ hist} v :
+    spsc_bqueue_history_auth γ hist ⊢ |==>
+    spsc_bqueue_history_auth γ (hist ++ [v]).
   Proof.
     apply mono_list_update_app.
   Qed.
 
-  #[local] Lemma spsc_queue_producer_ctl_alloc :
+  #[local] Lemma spsc_bqueue_producer_ctl_alloc :
     ⊢ |==>
       ∃ γ_producer_ctl,
-      spsc_queue_producer_ctl₁' γ_producer_ctl 0 ∗
-      spsc_queue_producer_ctl₂' γ_producer_ctl 0.
+      spsc_bqueue_producer_ctl₁' γ_producer_ctl 0 ∗
+      spsc_bqueue_producer_ctl₂' γ_producer_ctl 0.
   Proof.
     iMod auth_nat_max_alloc as "(%γ_producer_ctl & Hproducer_ctl₁ & Hproducer_ctl₂)".
     iSteps.
   Qed.
-  #[local] Lemma spsc_queue_producer_ctl_agree γ back1 back2 :
-    spsc_queue_producer_ctl₁ γ back1 -∗
-    spsc_queue_producer_ctl₂ γ back2 -∗
+  #[local] Lemma spsc_bqueue_producer_ctl_agree γ back1 back2 :
+    spsc_bqueue_producer_ctl₁ γ back1 -∗
+    spsc_bqueue_producer_ctl₂ γ back2 -∗
     ⌜back1 = back2⌝.
   Proof.
     apply auth_nat_max_auth_agree.
   Qed.
-  #[local] Lemma spsc_queue_producer_ctl_update {γ back1 back2} back :
+  #[local] Lemma spsc_bqueue_producer_ctl_update {γ back1 back2} back :
     back1 ≤ back →
-    spsc_queue_producer_ctl₁ γ back1 -∗
-    spsc_queue_producer_ctl₂ γ back2 ==∗
-      spsc_queue_producer_ctl₁ γ back ∗
-      spsc_queue_producer_ctl₂ γ back.
+    spsc_bqueue_producer_ctl₁ γ back1 -∗
+    spsc_bqueue_producer_ctl₂ γ back2 ==∗
+      spsc_bqueue_producer_ctl₁ γ back ∗
+      spsc_bqueue_producer_ctl₂ γ back.
   Proof.
     iIntros "%Hle Hproducer_ctl₁ Hproducer_ctl₂".
     iDestruct (auth_nat_max_auth_agree with "Hproducer_ctl₁ Hproducer_ctl₂") as %->.
     iCombine "Hproducer_ctl₁ Hproducer_ctl₂" as "Hproducer_ctl".
     iMod (auth_nat_max_update with "Hproducer_ctl") as "($ & $)"; done.
   Qed.
-  #[local] Lemma spsc_queue_back_lb_get γ back :
-    spsc_queue_producer_ctl₂ γ back ⊢
-    spsc_queue_back_lb γ back.
+  #[local] Lemma spsc_bqueue_back_lb_get γ back :
+    spsc_bqueue_producer_ctl₂ γ back ⊢
+    spsc_bqueue_back_lb γ back.
   Proof.
     apply auth_nat_max_lb_get.
   Qed.
-  #[local] Lemma spsc_queue_back_lb_valid γ back1 back2 :
-    spsc_queue_producer_ctl₂ γ back1 -∗
-    spsc_queue_back_lb γ back2 -∗
+  #[local] Lemma spsc_bqueue_back_lb_valid γ back1 back2 :
+    spsc_bqueue_producer_ctl₂ γ back1 -∗
+    spsc_bqueue_back_lb γ back2 -∗
     ⌜back2 ≤ back1⌝.
   Proof.
     apply auth_nat_max_lb_valid.
   Qed.
 
-  #[local] Lemma spsc_queue_producer_region_alloc :
+  #[local] Lemma spsc_bqueue_producer_region_alloc :
     ⊢ |==>
       ∃ γ_producer_region,
-      spsc_queue_producer_region' γ_producer_region.
+      spsc_bqueue_producer_region' γ_producer_region.
   Proof.
     apply excl_alloc.
   Qed.
-  #[local] Lemma spsc_queue_producer_region_exclusive γ :
-    spsc_queue_producer_region γ -∗
-    spsc_queue_producer_region γ -∗
+  #[local] Lemma spsc_bqueue_producer_region_exclusive γ :
+    spsc_bqueue_producer_region γ -∗
+    spsc_bqueue_producer_region γ -∗
     False.
   Proof.
     apply excl_exclusive.
   Qed.
 
-  #[local] Lemma spsc_queue_consumer_ctl_alloc :
+  #[local] Lemma spsc_bqueue_consumer_ctl_alloc :
     ⊢ |==>
       ∃ γ_consumer_ctl,
-      spsc_queue_consumer_ctl₁' γ_consumer_ctl 0 ∗
-      spsc_queue_consumer_ctl₂' γ_consumer_ctl 0.
+      spsc_bqueue_consumer_ctl₁' γ_consumer_ctl 0 ∗
+      spsc_bqueue_consumer_ctl₂' γ_consumer_ctl 0.
   Proof.
     iMod auth_nat_max_alloc as "(%γ_consumer_ctl & Hconsumer_ctl₁ & Hconsumer_ctl₂)".
     iSteps.
   Qed.
-  #[local] Lemma spsc_queue_consumer_ctl_agree γ front1 front2 :
-    spsc_queue_consumer_ctl₁ γ front1 -∗
-    spsc_queue_consumer_ctl₂ γ front2 -∗
+  #[local] Lemma spsc_bqueue_consumer_ctl_agree γ front1 front2 :
+    spsc_bqueue_consumer_ctl₁ γ front1 -∗
+    spsc_bqueue_consumer_ctl₂ γ front2 -∗
     ⌜front1 = front2⌝.
   Proof.
     apply auth_nat_max_auth_agree.
   Qed.
-  #[local] Lemma spsc_queue_consumer_ctl_update {γ front1 front2} front :
+  #[local] Lemma spsc_bqueue_consumer_ctl_update {γ front1 front2} front :
     front1 ≤ front →
-    spsc_queue_consumer_ctl₁ γ front1 -∗
-    spsc_queue_consumer_ctl₂ γ front2 ==∗
-      spsc_queue_consumer_ctl₁ γ front ∗
-      spsc_queue_consumer_ctl₂ γ front.
+    spsc_bqueue_consumer_ctl₁ γ front1 -∗
+    spsc_bqueue_consumer_ctl₂ γ front2 ==∗
+      spsc_bqueue_consumer_ctl₁ γ front ∗
+      spsc_bqueue_consumer_ctl₂ γ front.
   Proof.
     iIntros "%Hle Hconsumer_ctl₁ Hconsumer_ctl₂".
     iDestruct (auth_nat_max_auth_agree with "Hconsumer_ctl₁ Hconsumer_ctl₂") as %->.
     iCombine "Hconsumer_ctl₁ Hconsumer_ctl₂" as "Hconsumer_ctl".
     iMod (auth_nat_max_update with "Hconsumer_ctl") as "($ & $)"; done.
   Qed.
-  #[local] Lemma spsc_queue_front_lb_get γ front :
-    spsc_queue_consumer_ctl₂ γ front ⊢
-    spsc_queue_front_lb γ front.
+  #[local] Lemma spsc_bqueue_front_lb_get γ front :
+    spsc_bqueue_consumer_ctl₂ γ front ⊢
+    spsc_bqueue_front_lb γ front.
   Proof.
     apply auth_nat_max_lb_get.
   Qed.
-  #[local] Lemma spsc_queue_front_lb_valid γ front1 front2 :
-    spsc_queue_consumer_ctl₂ γ front1 -∗
-    spsc_queue_front_lb γ front2 -∗
+  #[local] Lemma spsc_bqueue_front_lb_valid γ front1 front2 :
+    spsc_bqueue_consumer_ctl₂ γ front1 -∗
+    spsc_bqueue_front_lb γ front2 -∗
     ⌜front2 ≤ front1⌝.
   Proof.
     iIntros "Hconsumer_ctl₁ Hfront_lb".
     iApply (auth_nat_max_lb_valid with "Hconsumer_ctl₁ Hfront_lb").
   Qed.
 
-  #[local] Lemma spsc_queue_consumer_region_alloc :
+  #[local] Lemma spsc_bqueue_consumer_region_alloc :
     ⊢ |==>
       ∃ γ_consumer_region,
-      spsc_queue_consumer_region' γ_consumer_region.
+      spsc_bqueue_consumer_region' γ_consumer_region.
   Proof.
     apply excl_alloc.
   Qed.
-  #[local] Lemma spsc_queue_consumer_region_exclusive γ :
-    spsc_queue_consumer_region γ -∗
-    spsc_queue_consumer_region γ -∗
+  #[local] Lemma spsc_bqueue_consumer_region_exclusive γ :
+    spsc_bqueue_consumer_region γ -∗
+    spsc_bqueue_consumer_region γ -∗
     False.
   Proof.
     apply excl_exclusive.
   Qed.
 
-  Lemma spsc_queue_producer_exclusive t :
-    spsc_queue_producer t -∗
-    spsc_queue_producer t -∗
+  Lemma spsc_bqueue_producer_exclusive t :
+    spsc_bqueue_producer t -∗
+    spsc_bqueue_producer t -∗
     False.
   Proof.
     iSteps.
   Qed.
 
-  Lemma spsc_queue_consumer_exclusive t :
-    spsc_queue_consumer t -∗
-    spsc_queue_consumer t -∗
+  Lemma spsc_bqueue_consumer_exclusive t :
+    spsc_bqueue_consumer t -∗
+    spsc_bqueue_consumer t -∗
     False.
   Proof.
     iSteps.
@@ -472,16 +472,16 @@ Section spsc_queue_G.
     iSteps. rewrite array_cslice_nil. iSteps.
   Qed.
 
-  Lemma spsc_queue_create_spec ι sz :
+  Lemma spsc_bqueue_create_spec ι sz :
     (0 ≤ sz)%Z →
     {{{ True }}}
-      spsc_queue_create #sz
+      spsc_bqueue_create #sz
     {{{ t,
       RET t;
-      spsc_queue_inv t ι (Z.to_nat sz) ∗
-      spsc_queue_model t [] ∗
-      spsc_queue_producer t ∗
-      spsc_queue_consumer t
+      spsc_bqueue_inv t ι (Z.to_nat sz) ∗
+      spsc_bqueue_model t [] ∗
+      spsc_bqueue_producer t ∗
+      spsc_bqueue_consumer t
     }}}.
   Proof.
     iIntros "%Hsz %Φ _ HΦ".
@@ -492,25 +492,25 @@ Section spsc_queue_G.
     wp_record l as "Hmeta" "(Hdata & Hfront & Hfront_cache & Hback & Hback_cache & _)".
     iMod (pointsto_persist with "Hdata") as "#Hdata".
 
-    iMod spsc_queue_model_alloc as "(%γ_model & Hmodel₁ & Hmodel₂)".
-    iMod spsc_queue_history_alloc as "(%γ_history & Hhistory_auth)".
-    iMod spsc_queue_producer_ctl_alloc as "(%γ_producer_ctl & Hproducer_ctl₁ & Hproducer_ctl₂)".
-    iMod spsc_queue_producer_region_alloc as "(%γ_producer_region & Hproducer_region)".
-    iMod spsc_queue_consumer_ctl_alloc as "(%γ_consumer_ctl & Hconsumer_ctl₁ & Hconsumer_ctl₂)".
-    iMod spsc_queue_consumer_region_alloc as "(%γ_consumer_region & Hconsumer_region)".
+    iMod spsc_bqueue_model_alloc as "(%γ_model & Hmodel₁ & Hmodel₂)".
+    iMod spsc_bqueue_history_alloc as "(%γ_history & Hhistory_auth)".
+    iMod spsc_bqueue_producer_ctl_alloc as "(%γ_producer_ctl & Hproducer_ctl₁ & Hproducer_ctl₂)".
+    iMod spsc_bqueue_producer_region_alloc as "(%γ_producer_region & Hproducer_region)".
+    iMod spsc_bqueue_consumer_ctl_alloc as "(%γ_consumer_ctl & Hconsumer_ctl₁ & Hconsumer_ctl₂)".
+    iMod spsc_bqueue_consumer_region_alloc as "(%γ_consumer_region & Hconsumer_region)".
 
     pose γ := {|
-      spsc_queue_meta_model := γ_model ;
-      spsc_queue_meta_history := γ_history ;
-      spsc_queue_meta_producer_ctl := γ_producer_ctl ;
-      spsc_queue_meta_producer_region := γ_producer_region ;
-      spsc_queue_meta_consumer_ctl := γ_consumer_ctl ;
-      spsc_queue_meta_consumer_region := γ_consumer_region ;
+      spsc_bqueue_meta_model := γ_model ;
+      spsc_bqueue_meta_history := γ_history ;
+      spsc_bqueue_meta_producer_ctl := γ_producer_ctl ;
+      spsc_bqueue_meta_producer_region := γ_producer_region ;
+      spsc_bqueue_meta_consumer_ctl := γ_consumer_ctl ;
+      spsc_bqueue_meta_consumer_region := γ_consumer_region ;
     |}.
     iMod (meta_set _ _ γ with "Hmeta") as "#Hmeta"; first done.
 
-    iDestruct (spsc_queue_back_lb_get γ with "Hproducer_ctl₂") as "#Hback_lb".
-    iDestruct (spsc_queue_front_lb_get γ with "Hconsumer_ctl₂") as "#Hfront_lb".
+    iDestruct (spsc_bqueue_back_lb_get γ with "Hproducer_ctl₂") as "#Hback_lb".
+    iDestruct (spsc_bqueue_front_lb_get γ with "Hconsumer_ctl₂") as "#Hfront_lb".
 
     iApply "HΦ".
     iSplitL "Hdata_model Hfront Hback Hmodel₂ Hhistory_auth Hproducer_ctl₂ Hconsumer_ctl₂"; last iSteps.
@@ -525,37 +525,37 @@ Section spsc_queue_G.
     rewrite Nat.sub_0_r. iSteps.
   Qed.
 
-  #[local] Definition spsc_queue_push_au l ι sz v Φ : iProp Σ :=
+  #[local] Definition spsc_bqueue_push_au l ι sz v Φ : iProp Σ :=
     AU <{
       ∃∃ vs,
-      spsc_queue_model #l vs
+      spsc_bqueue_model #l vs
     }> @ ⊤ ∖ ↑ι, ∅ <{
-      spsc_queue_model #l (if decide (length vs = sz) then vs else vs ++ [v]),
+      spsc_bqueue_model #l (if decide (length vs = sz) then vs else vs ++ [v]),
     COMM
-      spsc_queue_producer #l -∗
+      spsc_bqueue_producer #l -∗
       Φ #(bool_decide (length vs = sz))
     }>.
-  #[local] Lemma spsc_queue_push_aux_spec l ι γ sz data front_cache back v Ψ :
+  #[local] Lemma spsc_bqueue_push_aux_spec l ι γ sz data front_cache back v Ψ :
     {{{
       meta l nroot γ ∗
-      inv ι (spsc_queue_inv_inner l γ sz data) ∗
+      inv ι (spsc_bqueue_inv_inner l γ sz data) ∗
       array_inv data sz ∗
       l.[front_cache] ↦ #front_cache ∗
-      spsc_queue_producer_ctl₁ γ back ∗
-      spsc_queue_front_lb γ front_cache ∗
-      spsc_queue_push_au l ι sz v Ψ
+      spsc_bqueue_producer_ctl₁ γ back ∗
+      spsc_bqueue_front_lb γ front_cache ∗
+      spsc_bqueue_push_au l ι sz v Ψ
     }}}
-      spsc_queue_push_aux #l data #back
+      spsc_bqueue_push_aux #l data #back
     {{{ b front_cache',
       RET #b;
       ⌜b = bool_decide (back < front_cache' + sz)⌝ ∗
       l.[front_cache] ↦ #front_cache' ∗
-      spsc_queue_producer_ctl₁ γ back ∗
-      spsc_queue_front_lb γ front_cache' ∗
+      spsc_bqueue_producer_ctl₁ γ back ∗
+      spsc_bqueue_front_lb γ front_cache' ∗
       if b then
-        spsc_queue_push_au l ι sz v Ψ
+        spsc_bqueue_push_au l ι sz v Ψ
       else
-        spsc_queue_producer #l -∗
+        spsc_bqueue_producer #l -∗
         Ψ #true
     }}}.
   Proof.
@@ -572,8 +572,8 @@ Section spsc_queue_G.
     - wp_bind (!_)%E.
       iInv "Hinv" as "(%front & %_back & %vs & %hist & >(%Hback & %Hback_le) & >(%Hhist_len & %Hvs) & Hfront & Hconsumer_ctl₂ & Hback & Hproducer_ctl₂ & Hmodel₂ & Hhistory_auth & Hdata_front & Hdata_vs & Hdata_back & Hdata_extra)".
       wp_load.
-      iDestruct (spsc_queue_producer_ctl_agree with "Hproducer_ctl₁ Hproducer_ctl₂") as %<-.
-      iClear "Hfront_lb". iDestruct (spsc_queue_front_lb_get with "Hconsumer_ctl₂") as "#Hfront_lb".
+      iDestruct (spsc_bqueue_producer_ctl_agree with "Hproducer_ctl₁ Hproducer_ctl₂") as %<-.
+      iClear "Hfront_lb". iDestruct (spsc_bqueue_front_lb_get with "Hconsumer_ctl₂") as "#Hfront_lb".
       destruct (decide (back < front + sz)) as [Hbranch2 | Hbranch2].
 
       + iSplitR "Hfront_cache Hproducer_ctl₁ HΨ HΦ"; first iSteps.
@@ -585,7 +585,7 @@ Section spsc_queue_G.
 
       + iMod "HΨ" as "(%_vs & (%_l & %_γ & %Heq & _Hmeta & Hmodel₁) & _ & HΨ)". injection Heq as <-.
         iDestruct (meta_agree with "Hmeta _Hmeta") as %<-. iClear "_Hmeta".
-        iDestruct (spsc_queue_model_agree with "Hmodel₁ Hmodel₂") as %->.
+        iDestruct (spsc_bqueue_model_agree with "Hmodel₁ Hmodel₂") as %->.
         rewrite decide_True; [lia.. |]. rewrite bool_decide_eq_true_2; first lia.
         iMod ("HΨ" with "[Hmodel₁]") as "HΨ"; first iSteps.
         iSplitR "Hfront_cache Hproducer_ctl₁ HΨ HΦ"; first iSteps.
@@ -595,18 +595,18 @@ Section spsc_queue_G.
         iApply ("HΦ" $! _ front).
         rewrite !bool_decide_eq_false_2; [lia.. |]. iSteps.
   Qed.
-  Lemma spsc_queue_push_spec t ι sz v :
+  Lemma spsc_bqueue_push_spec t ι sz v :
     <<<
-      spsc_queue_inv t ι sz ∗
-      spsc_queue_producer t
+      spsc_bqueue_inv t ι sz ∗
+      spsc_bqueue_producer t
     | ∀∀ vs,
-      spsc_queue_model t vs
+      spsc_bqueue_model t vs
     >>>
-      spsc_queue_push t v @ ↑ι
+      spsc_bqueue_push t v @ ↑ι
     <<<
-      spsc_queue_model t (if decide (length vs = sz) then vs else vs ++ [v])
+      spsc_bqueue_model t (if decide (length vs = sz) then vs else vs ++ [v])
     | RET #(bool_decide (length vs = sz));
-      spsc_queue_producer t
+      spsc_bqueue_producer t
     >>>.
   Proof.
     iIntros "!> %Φ ((%l & %γ & %data & -> & #Hmeta & #Hdata & #Hinv) & (%_l & %_γ & %front_cache & %back & %Heq & #_Hmeta & Hfront_cache & Hproducer_ctl₁ & Hproducer_region & #Hfront_lb)) HΦ". injection Heq as <-.
@@ -617,20 +617,20 @@ Section spsc_queue_G.
     wp_bind (!_)%E.
     iInv "Hinv" as "(%front1 & %_back & %vs1 & %hist1 & >(%Hback & %Hback_le) & >(%Hhist1_len & %Hvs1) & Hfront & Hconsumer_ctl₂ & Hback & Hproducer_ctl₂ & Hmodel₂ & Hhistory_auth & Hdata_front & Hdata_vs & Hdata_back & Hdata_extra)".
     wp_load.
-    iDestruct (spsc_queue_producer_ctl_agree with "Hproducer_ctl₁ Hproducer_ctl₂") as %<-.
+    iDestruct (spsc_bqueue_producer_ctl_agree with "Hproducer_ctl₁ Hproducer_ctl₂") as %<-.
     iDestruct (array_cslice_to_inv with "Hdata_vs") as "#Hdata_inv".
     iSplitR "Hfront_cache Hproducer_ctl₁ Hproducer_region HΦ"; first iSteps.
     iModIntro. clear.
 
-    iDestruct "Hfront_lb" as "-#Hfront_lb". wp_smart_apply (spsc_queue_push_aux_spec with "[$]") as (? front_cache') "(-> & Hfront_cache & Hproducer_ctl₁ & #Hfront_lb & HΦ)".
+    iDestruct "Hfront_lb" as "-#Hfront_lb". wp_smart_apply (spsc_bqueue_push_aux_spec with "[$]") as (? front_cache') "(-> & Hfront_cache & Hproducer_ctl₁ & #Hfront_lb & HΦ)".
     case_bool_decide as Hbranch; last iSteps.
 
     iApply fupd_wp.
     iInv "Hinv" as "(%front2 & %_back & %vs2 & %hist2 & >(%Hback & %Hback_le) & >(%Hhist2_len & %Hvs2) & Hfront & >Hconsumer_ctl₂ & Hback & >Hproducer_ctl₂ & Hmodel₂ & Hhistory_auth & Hdata_front & Hdata_vs & >Hdata_back & Hdata_extra)".
-    iDestruct (spsc_queue_producer_ctl_agree with "Hproducer_ctl₁ Hproducer_ctl₂") as %<-.
+    iDestruct (spsc_bqueue_producer_ctl_agree with "Hproducer_ctl₁ Hproducer_ctl₂") as %<-.
     iDestruct "Hdata_back" as "[Hdata_back | Hproducer_region']"; last first.
-    { iDestruct (spsc_queue_producer_region_exclusive with "Hproducer_region Hproducer_region'") as %[]. }
-    iDestruct (spsc_queue_front_lb_valid with "Hconsumer_ctl₂ Hfront_lb") as %Hfront2.
+    { iDestruct (spsc_bqueue_producer_region_exclusive with "Hproducer_region Hproducer_region'") as %[]. }
+    iDestruct (spsc_bqueue_front_lb_valid with "Hconsumer_ctl₂ Hfront_lb") as %Hfront2.
     rewrite decide_False; first lia.
     iSplitR "Hfront_cache Hproducer_ctl₁ Hdata_back HΦ"; first iSteps.
     iModIntro. clear- Hbranch. iModIntro.
@@ -641,18 +641,18 @@ Section spsc_queue_G.
     wp_bind (_ <- _)%E.
     iInv "Hinv" as "(%front3 & %_back & %vs3 & %hist3 & >(%Hback & %Hback_le) & >(%Hhist3_len & %Hvs3) & Hfront & Hconsumer_ctl₂ & Hback & Hproducer_ctl₂ & Hmodel₂ & Hhistory_auth & Hdata_front & Hdata_vs & Hproducer_region & Hdata_extra)".
     wp_store.
-    iDestruct (spsc_queue_producer_ctl_agree with "Hproducer_ctl₁ Hproducer_ctl₂") as %<-.
-    iDestruct (spsc_queue_front_lb_valid with "Hconsumer_ctl₂ Hfront_lb") as %Hfront3_ge.
+    iDestruct (spsc_bqueue_producer_ctl_agree with "Hproducer_ctl₁ Hproducer_ctl₂") as %<-.
+    iDestruct (spsc_bqueue_front_lb_valid with "Hconsumer_ctl₂ Hfront_lb") as %Hfront3_ge.
     iDestruct "Hproducer_region" as "[Hdata_back' | Hproducer_region]".
     { rewrite decide_False; first lia.
       iDestruct (array_cslice_exclusive with "Hdata_back Hdata_back'") as %[]; [simpl; lia | done].
     }
-    iMod (spsc_queue_producer_ctl_update (S back) with "Hproducer_ctl₁ Hproducer_ctl₂") as "(Hproducer_ctl₁ & Hproducer_ctl₂)"; first lia.
-    iMod (spsc_queue_history_update v with "Hhistory_auth") as "Hhistory_auth".
+    iMod (spsc_bqueue_producer_ctl_update (S back) with "Hproducer_ctl₁ Hproducer_ctl₂") as "(Hproducer_ctl₁ & Hproducer_ctl₂)"; first lia.
+    iMod (spsc_bqueue_history_update v with "Hhistory_auth") as "Hhistory_auth".
     iMod "HΦ" as "(%vs & (%_l & %_γ & %Heq & _Hmeta & Hmodel₁) & _ & HΦ)". injection Heq as <-.
     iDestruct (meta_agree with "Hmeta _Hmeta") as %<-. iClear "_Hmeta".
-    iDestruct (spsc_queue_model_agree with "Hmodel₁ Hmodel₂") as %->.
-    iMod (spsc_queue_model_update (vs3 ++ [v]) with "Hmodel₁ Hmodel₂") as "(Hmodel₁ & Hmodel₂)".
+    iDestruct (spsc_bqueue_model_agree with "Hmodel₁ Hmodel₂") as %->.
+    iMod (spsc_bqueue_model_update (vs3 ++ [v]) with "Hmodel₁ Hmodel₂") as "(Hmodel₁ & Hmodel₂)".
     rewrite decide_False; first lia.
     iMod ("HΦ" with "[Hmodel₁]") as "HΦ"; first iSteps.
     rewrite bool_decide_eq_false_2; first lia.
@@ -678,36 +678,36 @@ Section spsc_queue_G.
     iSteps.
   Qed.
 
-  #[local] Definition spsc_queue_pop_au l ι Φ : iProp Σ :=
+  #[local] Definition spsc_bqueue_pop_au l ι Φ : iProp Σ :=
     AU <{
       ∃∃ vs,
-      spsc_queue_model #l vs
+      spsc_bqueue_model #l vs
     }> @ ⊤ ∖ ↑ι, ∅ <{
-      spsc_queue_model #l (tail vs),
+      spsc_bqueue_model #l (tail vs),
     COMM
-      spsc_queue_consumer #l -∗
+      spsc_bqueue_consumer #l -∗
       Φ (head vs : val)
     }>.
-  #[local] Lemma spsc_queue_pop_aux_spec l ι γ sz data front back_cache Ψ :
+  #[local] Lemma spsc_bqueue_pop_aux_spec l ι γ sz data front back_cache Ψ :
     {{{
       meta l nroot γ ∗
-      inv ι (spsc_queue_inv_inner l γ sz data) ∗
+      inv ι (spsc_bqueue_inv_inner l γ sz data) ∗
       l.[back_cache] ↦ #back_cache ∗
-      spsc_queue_consumer_ctl₁ γ front ∗
-      spsc_queue_back_lb γ back_cache ∗
-      spsc_queue_pop_au l ι Ψ
+      spsc_bqueue_consumer_ctl₁ γ front ∗
+      spsc_bqueue_back_lb γ back_cache ∗
+      spsc_bqueue_pop_au l ι Ψ
     }}}
-      spsc_queue_pop_aux #l #front
+      spsc_bqueue_pop_aux #l #front
     {{{ b back_cache',
       RET #b;
       ⌜b = bool_decide (front < back_cache')⌝ ∗
       l.[back_cache] ↦ #back_cache' ∗
-      spsc_queue_consumer_ctl₁ γ front ∗
-      spsc_queue_back_lb γ back_cache' ∗
+      spsc_bqueue_consumer_ctl₁ γ front ∗
+      spsc_bqueue_back_lb γ back_cache' ∗
       if b then
-        spsc_queue_pop_au l ι Ψ
+        spsc_bqueue_pop_au l ι Ψ
       else
-        spsc_queue_consumer #l -∗
+        spsc_bqueue_consumer #l -∗
         Ψ None
     }}}.
   Proof.
@@ -723,8 +723,8 @@ Section spsc_queue_G.
     - wp_bind (!_)%E.
       iInv "Hinv" as "(%_front & %back & %vs & %hist & >(%Hback & %Hback_le) & >(%Hhist_len & %Hvs) & Hfront & Hconsumer_ctl₂ & Hback & Hproducer_ctl₂ & Hmodel₂ & Hhistory_auth & Hdata_front & Hdata_vs & Hdata_back & Hdata_extra)".
       wp_load.
-      iDestruct (spsc_queue_consumer_ctl_agree with "Hconsumer_ctl₁ Hconsumer_ctl₂") as %<-.
-      iClear "Hback_lb". iDestruct (spsc_queue_back_lb_get with "Hproducer_ctl₂") as "#Hback_lb".
+      iDestruct (spsc_bqueue_consumer_ctl_agree with "Hconsumer_ctl₁ Hconsumer_ctl₂") as %<-.
+      iClear "Hback_lb". iDestruct (spsc_bqueue_back_lb_get with "Hproducer_ctl₂") as "#Hback_lb".
       destruct (decide (front < back)) as [Hbranch2 | Hbranch2].
 
       + iSplitR "Hback_cache Hconsumer_ctl₁ HΨ HΦ".
@@ -738,7 +738,7 @@ Section spsc_queue_G.
       + assert (front = back) as <- by lia.
         iMod "HΨ" as "(%_vs & (%_l & %_γ & %Heq & _Hmeta & Hmodel₁) & _ & HΨ)". injection Heq as <-.
         iDestruct (meta_agree with "Hmeta _Hmeta") as %<-. iClear "_Hmeta".
-        iDestruct (spsc_queue_model_agree with "Hmodel₁ Hmodel₂") as %->.
+        iDestruct (spsc_bqueue_model_agree with "Hmodel₁ Hmodel₂") as %->.
         assert (length vs = 0) as ->%nil_length_inv by lia.
         iMod ("HΨ" with "[Hmodel₁]") as "HΨ"; first iSteps.
         iSplitR "Hback_cache Hconsumer_ctl₁ HΨ HΦ"; first iSteps.
@@ -748,18 +748,18 @@ Section spsc_queue_G.
         iApply ("HΦ" $! _ front).
         rewrite !bool_decide_eq_false_2; [lia.. |]. iSteps.
   Qed.
-  Lemma spsc_queue_pop_spec t ι sz :
+  Lemma spsc_bqueue_pop_spec t ι sz :
     <<<
-      spsc_queue_inv t ι sz ∗
-      spsc_queue_consumer t
+      spsc_bqueue_inv t ι sz ∗
+      spsc_bqueue_consumer t
     | ∀∀ vs,
-      spsc_queue_model t vs
+      spsc_bqueue_model t vs
     >>>
-      spsc_queue_pop t @ ↑ι
+      spsc_bqueue_pop t @ ↑ι
     <<<
-      spsc_queue_model t (tail vs)
+      spsc_bqueue_model t (tail vs)
     | RET head vs;
-      spsc_queue_consumer t
+      spsc_bqueue_consumer t
     >>>.
   Proof.
     iIntros "!> %Φ ((%l & %γ & %data & -> & #Hmeta & #Hdata & #Hinv) & (%_l & %_γ & %front & %back_cache & %Heq & #_Hmeta & Hback_cache & Hconsumer_ctl₁ & Hconsumer_region & #Hback_lb)) HΦ". injection Heq as <-.
@@ -770,23 +770,23 @@ Section spsc_queue_G.
     wp_bind (!_)%E.
     iInv "Hinv" as "(%_front & %back1 & %vs1 & %hist1 & >(%Hback1 & %Hback1_le) & >(%Hhist1_len & %Hvs1) & Hfront & Hconsumer_ctl₂ & Hback & Hproducer_ctl₂ & Hmodel₂ & Hhistory_auth & Hdata_front & Hdata_vs & Hdata_back & Hdata_extra)".
     wp_load.
-    iDestruct (spsc_queue_consumer_ctl_agree with "Hconsumer_ctl₁ Hconsumer_ctl₂") as %<-.
+    iDestruct (spsc_bqueue_consumer_ctl_agree with "Hconsumer_ctl₁ Hconsumer_ctl₂") as %<-.
     iDestruct (array_cslice_to_inv with "Hdata_vs") as "#Hdata_inv".
     iSplitR "Hback_cache Hconsumer_ctl₁ Hconsumer_region HΦ".
     { iExists front, back1, vs1, hist1. iSteps. }
     iModIntro. clear.
 
-    iDestruct "Hback_lb" as "-#Hback_lb". wp_smart_apply (spsc_queue_pop_aux_spec with "[$]") as (? back_cache') "(-> & Hback_cache & Hconsumer_ctl₁ & #Hback_lb & HΦ)".
+    iDestruct "Hback_lb" as "-#Hback_lb". wp_smart_apply (spsc_bqueue_pop_aux_spec with "[$]") as (? back_cache') "(-> & Hback_cache & Hconsumer_ctl₁ & #Hback_lb & HΦ)".
     case_bool_decide as Hbranch; last iSteps.
 
     iApply fupd_wp.
     iInv "Hinv" as "(%_front & %back2 & %vs2 & %hist2 & >(%Hback2 & %Hback2_le) & >(%Hhist2_len & %Hvs2) & Hfront & >Hconsumer_ctl₂ & Hback & >Hproducer_ctl₂ & Hmodel₂ & Hhistory_auth & >Hdata_front & Hdata_vs & Hdata_back & Hdata_extra)".
-    iDestruct (spsc_queue_consumer_ctl_agree with "Hconsumer_ctl₁ Hconsumer_ctl₂") as %<-.
-    iDestruct (spsc_queue_back_lb_valid with "Hproducer_ctl₂ Hback_lb") as %Hback2_ge.
+    iDestruct (spsc_bqueue_consumer_ctl_agree with "Hconsumer_ctl₁ Hconsumer_ctl₂") as %<-.
+    iDestruct (spsc_bqueue_back_lb_valid with "Hproducer_ctl₂ Hback_lb") as %Hback2_ge.
     destruct vs2 as [| v vs2]; first naive_solver lia.
     iDestruct "Hdata_front" as "[Hdata_front | Hconsumer_region']"; last first.
-    { iDestruct (spsc_queue_consumer_region_exclusive with "Hconsumer_region Hconsumer_region'") as %[]. }
-    iDestruct (spsc_queue_history_elem_get front v with "Hhistory_auth") as "#Hhistory_elem".
+    { iDestruct (spsc_bqueue_consumer_region_exclusive with "Hconsumer_region Hconsumer_region'") as %[]. }
+    iDestruct (spsc_bqueue_history_elem_get front v with "Hhistory_auth") as "#Hhistory_elem".
     { rewrite -(take_drop front hist2) -Hvs2 lookup_app_r take_length; first lia.
       rewrite Nat.min_l; first lia.
       rewrite Nat.sub_diag //.
@@ -803,10 +803,10 @@ Section spsc_queue_G.
     wp_bind (_ <- _)%E.
     iInv "Hinv" as "(%_front & %back3 & %vs3 & %hist3 & >(%Hback3 & %Hback3_le) & >(%Hhist3_len & %Hvs3) & Hfront & Hconsumer_ctl₂ & Hback & Hproducer_ctl₂ & Hmodel₂ & Hhistory_auth & Hconsumer_region & Hdata_vs & Hdata_back & Hdata_extra)".
     wp_store.
-    iDestruct (spsc_queue_consumer_ctl_agree with "Hconsumer_ctl₁ Hconsumer_ctl₂") as %<-.
-    iDestruct (spsc_queue_back_lb_valid with "Hproducer_ctl₂ Hback_lb") as %Hback2.
+    iDestruct (spsc_bqueue_consumer_ctl_agree with "Hconsumer_ctl₁ Hconsumer_ctl₂") as %<-.
+    iDestruct (spsc_bqueue_back_lb_valid with "Hproducer_ctl₂ Hback_lb") as %Hback2.
     destruct vs3 as [| _v vs3]; first naive_solver lia.
-    iDestruct (spsc_queue_history_agree with "Hhistory_auth Hhistory_elem") as %Hhist3_lookup.
+    iDestruct (spsc_bqueue_history_agree with "Hhistory_auth Hhistory_elem") as %Hhist3_lookup.
     assert (_v = v) as ->.
     { move: Hhist3_lookup.
       rewrite -(take_drop front hist3) -Hvs3 lookup_app_r take_length; first lia.
@@ -816,11 +816,11 @@ Section spsc_queue_G.
     rewrite /= drop_0.
     iDestruct "Hconsumer_region" as "[Hdata_front' | Hconsumer_region]".
     { iDestruct (array_cslice_exclusive with "Hdata_front Hdata_front'") as %[]; [simpl; lia | done]. }
-    iMod (spsc_queue_consumer_ctl_update (S front) with "Hconsumer_ctl₁ Hconsumer_ctl₂") as "(Hconsumer_ctl₁ & Hconsumer_ctl₂)"; first lia.
+    iMod (spsc_bqueue_consumer_ctl_update (S front) with "Hconsumer_ctl₁ Hconsumer_ctl₂") as "(Hconsumer_ctl₁ & Hconsumer_ctl₂)"; first lia.
     iMod "HΦ" as "(%vs & (%_l & %_γ & %Heq & _Hmeta & Hmodel₁) & _ & HΦ)". injection Heq as <-.
     iDestruct (meta_agree with "Hmeta _Hmeta") as %<-. iClear "_Hmeta".
-    iDestruct (spsc_queue_model_agree with "Hmodel₁ Hmodel₂") as %->.
-    iMod (spsc_queue_model_update vs3 with "Hmodel₁ Hmodel₂") as "(Hmodel₁ & Hmodel₂)".
+    iDestruct (spsc_bqueue_model_agree with "Hmodel₁ Hmodel₂") as %->.
+    iMod (spsc_bqueue_model_update vs3 with "Hmodel₁ Hmodel₂") as "(Hmodel₁ & Hmodel₂)".
     iMod ("HΦ" with "[Hmodel₁]") as "HΦ"; first iSteps.
     iSplitR "Hback_cache Hconsumer_ctl₁ Hconsumer_region HΦ".
     { do 2 iModIntro. iExists (S front), back3, vs3, hist3. iFrame. simpl in *.
@@ -845,13 +845,13 @@ Section spsc_queue_G.
     }
     iSteps.
   Qed.
-End spsc_queue_G.
+End spsc_bqueue_G.
 
-#[global] Opaque spsc_queue_create.
-#[global] Opaque spsc_queue_push.
-#[global] Opaque spsc_queue_pop.
+#[global] Opaque spsc_bqueue_create.
+#[global] Opaque spsc_bqueue_push.
+#[global] Opaque spsc_bqueue_pop.
 
-#[global] Opaque spsc_queue_inv.
-#[global] Opaque spsc_queue_model.
-#[global] Opaque spsc_queue_producer.
-#[global] Opaque spsc_queue_consumer.
+#[global] Opaque spsc_bqueue_inv.
+#[global] Opaque spsc_bqueue_model.
+#[global] Opaque spsc_bqueue_producer.
+#[global] Opaque spsc_bqueue_consumer.
